backend/Lineartyping.v
@@ -133,7 +133,7 @@ Inductive wt_fundef: fundef -> Prop :=
       wt_fundef (Internal f).
 
 Definition wt_program (p: program) : Prop :=
-  forall i f, In (i, f) (prog_funct p) -> wt_fundef f.
+  forall i f, In (i, Gfun f) (prog_defs p) -> wt_fundef f.
 
 (** Typing the run-time state.  These definitions are used in [Stackingproof]. *)
 
